rocq-osiris/interp/O2E.ml
@@ -143,7 +143,6 @@ let rec expr : O.expr -> E.expr = function
   | EStore (e1, e2) -> EStore (expr e1, expr e2)
   | EFork (e1, e2) -> EFork (expr e1, expr e2)
   | EJoin e -> EJoin (expr e)
-  | ESelf -> ESelf
 
 and fexpr : O.fexpr -> E.fexpr = function
   Fexpr (f, e) -> Fexpr (field f, expr e)
