rocq-osiris/theories/program_logic/program_logic.v
@@ -8,6 +8,7 @@ From osiris.program_logic Require Export
   handler_rules
   fun_spec
   reasoning_rules.expr_rules
+  impure_rules
 .
 
 From osiris.program_logic.pure Require Export pure.
