rocq-osiris/theories/program_logic/reasoning_rules/expr_rules.v
@@ -6,7 +6,7 @@ From osiris.program_logic.reasoning_rules Require Import basic_rules impure_rule
 Section imp_rules_expr.
 
   Context `{!osirisGS Σ}.
-  Context {ι : thread} {E : coPset} {Ψ : iEff Σ}.
+  Context {E : coPset} {Ψ : iEff Σ}.
   Context {A : Type} `{EncA : Encode A} {Φ : A → iProp Σ}.
 
   (* -------------------------------------------------------------------------- *)
@@ -15,8 +15,8 @@ Section imp_rules_expr.
   (** * EPath : path → expr *)
 
   Lemma imp_EPath {ζ} η p :
-    imp^{ι} lookup_path η p @ E <|Ψ|> {{ Φ }} -∗
-    imp^{ι} eval η (EPath p) @ E <|Ψ|> ⟨⟨ ζ ⟩⟩ {{ Φ }}.
+    imp lookup_path η p @ E <|Ψ|> {{ Φ }} -∗
+    imp eval η (EPath p) @ E <|Ψ|> ⟨⟨ ζ ⟩⟩ {{ Φ }}.
   Proof.
     iIntros "H /=". simpl_eval.
     iApply (imp_widen with "H").
@@ -27,12 +27,12 @@ Section imp_rules_expr.
   (* See [funspec.v] *)
 
   Lemma imp_EApp_exn `{Encode B} {ζ} η e1 e2 ζ1 Φ1 ζ2 (Φ2 : B → iProp Σ) :
-    imp^{ι} eval η e1 @ E <|Ψ|> ⟨⟨ ζ1 ⟩⟩ {{ Φ1 }} -∗
-    imp^{ι} eval η e2 @ E <|Ψ|> ⟨⟨ ζ2 ⟩⟩ {{ Φ2 }} -∗
+    imp eval η e1 @ E <|Ψ|> ⟨⟨ ζ1 ⟩⟩ {{ Φ1 }} -∗
+    imp eval η e2 @ E <|Ψ|> ⟨⟨ ζ2 ⟩⟩ {{ Φ2 }} -∗
     ▷ (∀ e, ζ1 e -∗ ζ e) ∧
     ▷ (∀ e, ζ2 e -∗ ζ e) ∧
-    ▷ (∀ f x, Φ1 f -∗ Φ2 x -∗ imp^{ι} call f #x @ E <|Ψ|> ⟨⟨ ζ ⟩⟩ {{ Φ }}) -∗
-    imp^{ι} eval η (EApp e1 e2) @ E <|Ψ|> ⟨⟨ ζ ⟩⟩ {{ Φ }}.
+    ▷ (∀ f x, Φ1 f -∗ Φ2 x -∗ imp call f #x @ E <|Ψ|> ⟨⟨ ζ ⟩⟩ {{ Φ }}) -∗
+    imp eval η (EApp e1 e2) @ E <|Ψ|> ⟨⟨ ζ ⟩⟩ {{ Φ }}.
   Proof.
     iIntros "H1 H2 Hjoin /=". simpl_eval.
     iApply (imp_Par with "H1 H2").
@@ -47,10 +47,10 @@ Section imp_rules_expr.
   Qed.
 
   Lemma imp_EApp' `{Encode B} {ζ} η e1 e2 Φ1 (Φ2 : B → iProp Σ) :
-    imp^{ι} eval η e1 @ E <|Ψ|> {{ Φ1 }} -∗
-    imp^{ι} eval η e2 @ E <|Ψ|> {{ Φ2 }} -∗
-    ▷ (∀ f x, Φ1 f -∗ Φ2 x -∗ imp^{ι} call f #x @ E <|Ψ|> ⟨⟨ ζ ⟩⟩ {{ Φ }}) -∗
-    imp^{ι} eval η (EApp e1 e2) @ E <|Ψ|> ⟨⟨ ζ ⟩⟩ {{ Φ }}.
+    imp eval η e1 @ E <|Ψ|> {{ Φ1 }} -∗
+    imp eval η e2 @ E <|Ψ|> {{ Φ2 }} -∗
+    ▷ (∀ f x, Φ1 f -∗ Φ2 x -∗ imp call f #x @ E <|Ψ|> ⟨⟨ ζ ⟩⟩ {{ Φ }}) -∗
+    imp eval η (EApp e1 e2) @ E <|Ψ|> ⟨⟨ ζ ⟩⟩ {{ Φ }}.
   Proof.
     iIntros "H1 H2 H".
     iApply (imp_EApp_exn with "H1 H2").
@@ -68,8 +68,8 @@ Section imp_rules_expr.
   might be too verbose or be too trivial, and one could simply wish to "just
   reduce" the term, in which case those lemmas may be useful. *)
   Lemma imp_call_nonrec {ζ} η x_arg body v_arg :
-    ▷imp^{ι} eval ((x_arg, v_arg) :: η) body @ E <|Ψ|> ⟨⟨ ζ ⟩⟩ {{ Φ }} -∗
-    imp^{ι} call (VClo η (AnonFun x_arg body)) v_arg @ E <|Ψ|> ⟨⟨ ζ ⟩⟩ {{ Φ }}.
+    ▷imp eval ((x_arg, v_arg) :: η) body @ E <|Ψ|> ⟨⟨ ζ ⟩⟩ {{ Φ }} -∗
+    imp call (VClo η (AnonFun x_arg body)) v_arg @ E <|Ψ|> ⟨⟨ ζ ⟩⟩ {{ Φ }}.
   Proof.
     iIntros "H".
     by iApply imp_please.
@@ -77,8 +77,8 @@ Section imp_rules_expr.
 
   Lemma imp_call_rec {ζ} η f x body bs v :
     lookup_rec_bindings bs f = ret (AnonFun x body) ->
-    ▷ imp^{ι} eval ((x, v) :: eval_rec_bindings η bs ++ η) body @ E <|Ψ|> ⟨⟨ ζ ⟩⟩ {{ Φ }} -∗
-    imp^{ι} call (VCloRec η bs f) v @ E <|Ψ|> ⟨⟨ ζ ⟩⟩ {{ Φ }}.
+    ▷ imp eval ((x, v) :: eval_rec_bindings η bs ++ η) body @ E <|Ψ|> ⟨⟨ ζ ⟩⟩ {{ Φ }} -∗
+    imp call (VCloRec η bs f) v @ E <|Ψ|> ⟨⟨ ζ ⟩⟩ {{ Φ }}.
   Proof.
     iIntros (Hlk) "H /=". rewrite Hlk /=.
     by iApply imp_please.
@@ -88,8 +88,8 @@ Section imp_rules_expr.
 
   Lemma imp_evals {ζ} η es (Φs : list (val → iProp Σ)) :
     ([∗ list] ei;Φi ∈ es;Φs,
-       imp^{ι} eval η ei @ E <|Ψ|> ⟨⟨ ζ ⟩⟩ {{ Φi }}) -∗
-    imp^{ι} evals η es @ E <|Ψ|> ⟨⟨ ζ ⟩⟩
+       imp eval η ei @ E <|Ψ|> ⟨⟨ ζ ⟩⟩ {{ Φi }}) -∗
+    imp evals η es @ E <|Ψ|> ⟨⟨ ζ ⟩⟩
           {{ λ (vs : list val), [∗ list] vi; Φi ∈ vs; Φs, Φi vi }}.
   Proof.
     iIntros "HΦs".
@@ -113,8 +113,8 @@ Section imp_rules_expr.
 
   Lemma imp_ETuple_forward_exn {ζ} η es (Φs : list (val → iProp Σ)) :
     ([∗ list] ei; Φi ∈ es; Φs,
-       imp^{ι} eval η ei @ E <|Ψ|> ⟨⟨ ζ ⟩⟩ {{ Φi }}) -∗
-    imp^{ι} eval η (ETuple es) @ E <|Ψ|> ⟨⟨ ζ ⟩⟩
+       imp eval η ei @ E <|Ψ|> ⟨⟨ ζ ⟩⟩ {{ Φi }}) -∗
+    imp eval η (ETuple es) @ E <|Ψ|> ⟨⟨ ζ ⟩⟩
           {{ λ v, ∃ vs, ⌜v = VTuple vs⌝ ∗ [∗ list] vi; Φi ∈ vs; Φs, Φi vi }}.
   Proof.
     iIntros "H /=". simpl_eval.
@@ -129,8 +129,8 @@ Section imp_rules_expr.
 
   Lemma imp_ETuple_forward η es (Φs : list (val → iProp Σ)) :
     ([∗ list] ei; Φi ∈ es; Φs,
-       imp^{ι} eval η ei @ E <|Ψ|> {{ Φi }}) -∗
-    imp^{ι} eval η (ETuple es) @ E <|Ψ|>
+       imp eval η ei @ E <|Ψ|> {{ Φi }}) -∗
+    imp eval η (ETuple es) @ E <|Ψ|>
       {{ λ v, ∃ vs, ⌜v = VTuple vs⌝ ∗ [∗ list] vi; Φi ∈ vs; Φs, Φi vi }}.
   Proof.
     iIntros "Himps".
@@ -139,11 +139,11 @@ Section imp_rules_expr.
 
   Lemma imp_ETuple_exn {ζ} η es ζs Φs :
     ([∗ list] ei; '(ζi, Φi) ∈ es; zip ζs Φs,
-       imp^{ι} eval η ei @ E <|Ψ|> ⟨⟨ ζi ⟩⟩ {{ Φi }}) -∗
+       imp eval η ei @ E <|Ψ|> ⟨⟨ ζi ⟩⟩ {{ Φi }}) -∗
     (∀ vs, ([∗ list] vi; Φi ∈ vs; Φs, Φi vi) -∗
            ∃ a, ⌜#a = VTuple vs⌝ ∗ Φ a) -∗
     ([∗ list] ζi ∈ ζs, ∀ e, ζi e -∗ ζ e) -∗
-    imp^{ι} eval η (ETuple es) @ E <|Ψ|> ⟨⟨ ζ ⟩⟩ {{ Φ }}.
+    imp eval η (ETuple es) @ E <|Ψ|> ⟨⟨ ζ ⟩⟩ {{ Φ }}.
   Proof.
     iIntros "H P E". simpl_eval.
     iApply (imp_bind _ _ (λ vs, ret (VTuple vs)) with "[- P]").
@@ -163,7 +163,7 @@ Section imp_rules_expr.
   (* Results to handle goals generated by imp_ETuple_* lemmas *)
   Lemma imp_list_nil η  :
     ⊢ ([∗ list] ei;Φi ∈ []; @nil (val → iProp Σ),
-         imp^{ι} eval η ei @ E <|Ψ|> {{ Φi }}).
+         imp eval η ei @ E <|Ψ|> {{ Φi }}).
   Proof. done. Qed.
 
   (* Lemma imp_ETuple {ζ} η es Φs : *)
@@ -191,29 +191,29 @@ End imp_rules_expr.
 Section imp_rules_expr.
 
   Context `{!osirisGS Σ}.
-  Context {ι : thread} {E : coPset} {Ψ : iEff Σ}.
+  Context {E : coPset} {Ψ : iEff Σ}.
 
   Lemma imp_EUnit_exn {Φ ζ} η :
     Φ tt -∗
-    imp^{ι}eval η EUnit @ E <|Ψ|> ⟨⟨ ζ ⟩⟩ {{ Φ }}.
+    imp eval η EUnit @ E <|Ψ|> ⟨⟨ ζ ⟩⟩ {{ Φ }}.
   Proof.
     simpl_eval; by iApply imp_ret.
   Qed.
 
   Lemma imp_EUnit_forward {ζ} η :
-    ⊢ imp^{ι} eval η EUnit @ E <|Ψ|> ⟨⟨ ζ ⟩⟩ {{ λ u, ⌜u = tt⌝ }}.
+    ⊢ imp eval η EUnit @ E <|Ψ|> ⟨⟨ ζ ⟩⟩ {{ λ u, ⌜u = tt⌝ }}.
   Proof.
     simpl_eval; iApply imp_ret; [ encode | auto ].
   Qed.
 
   Lemma imp_EPair2 `{Encode A, Encode B} {ζ Φ} η e1 e2 ζ1 ζ2 (Φ1 : A → iProp Σ) (Φ2 : B → iProp Σ) :
-    imp^{ι} eval η e1 @ E <|Ψ|> ⟨⟨ ζ1 ⟩⟩ {{ Φ1 }} -∗
-    imp^{ι} eval η e2 @ E <|Ψ|> ⟨⟨ ζ2 ⟩⟩ {{ Φ2 }} -∗
+    imp eval η e1 @ E <|Ψ|> ⟨⟨ ζ1 ⟩⟩ {{ Φ1 }} -∗
+    imp eval η e2 @ E <|Ψ|> ⟨⟨ ζ2 ⟩⟩ {{ Φ2 }} -∗
     (∀ e, ζ1 e -∗ ζ e) ∧
     (∀ e, ζ2 e -∗ ζ e) ∧
     (∀ a1 a2, Φ1 a1 -∗ Φ2 a2 -∗
               Φ (a1, a2)) -∗
-    imp^{ι} eval η (EPair e1 e2) @ E <|Ψ|> ⟨⟨ ζ ⟩⟩ {{ Φ }}.
+    imp eval η (EPair e1 e2) @ E <|Ψ|> ⟨⟨ ζ ⟩⟩ {{ Φ }}.
   Proof.
     iIntros "H1 H2 Hjoin". simpl_eval.
     iApply (imp_Par Φ1 ζ1 _ _ _
@@ -227,7 +227,7 @@ Section imp_rules_expr.
     { iSplit; last iSplit.
       - iIntros (e) "Hζ2 !>".
         rewrite /discontinue /=.
-        iApply (@imp_throw Σ osirisGS0 (list B) (list val) exn _ _ ι E Ψ ζ2 _ e).
+        iApply (@imp_throw Σ osirisGS0 (list B) (list val) exn _ _ E Ψ ζ2 _ e).
         iExact "Hζ2".
       - iIntros (e). instantiate (2 := (λ _, False)%I).
         iIntros ([]).
@@ -250,10 +250,10 @@ Section imp_rules_expr.
   Qed.
 
   Lemma imp_EPair `{Encode A, Encode B} {Φ} η e1 e2 (Φ1 : A → iProp Σ) (Φ2 : B → iProp Σ) :
-    imp^{ι} eval η e1 @ E <|Ψ|> {{ Φ1 }} -∗
-    imp^{ι} eval η e2 @ E <|Ψ|> {{ Φ2 }} -∗
+    imp eval η e1 @ E <|Ψ|> {{ Φ1 }} -∗
+    imp eval η e2 @ E <|Ψ|> {{ Φ2 }} -∗
     (∀ a b, Φ1 a -∗ Φ2 b -∗ Φ (a, b)) -∗
-    imp^{ι} eval η (EPair e1 e2) @ E <|Ψ|> {{ Φ }}.
+    imp eval η (EPair e1 e2) @ E <|Ψ|> {{ Φ }}.
   Proof.
     iIntros "H1 H2 P".
     iApply (imp_EPair2 with "H1 H2 [P]"); auto.
@@ -263,11 +263,11 @@ Section imp_rules_expr.
 
   Lemma imp_EData `{Encode A} {Φ : A → iProp Σ} {ζ} η c es Φs :
     ([∗ list] ei;Φi ∈ es;Φs,
-       imp^{ι} eval η ei @ E <|Ψ|> ⟨⟨ ζ ⟩⟩ {{ Φi }}) -∗
+       imp eval η ei @ E <|Ψ|> ⟨⟨ ζ ⟩⟩ {{ Φi }}) -∗
     (∀ vs,
        ([∗ list] vi;Φi ∈ vs;Φs, Φi vi) -∗
        ∃ a, ⌜#a = VData c vs⌝ ∗ Φ a) -∗
-    imp^{ι} eval η (EData c es) @ E <|Ψ|> ⟨⟨ ζ ⟩⟩ {{ Φ }}.
+    imp eval η (EData c es) @ E <|Ψ|> ⟨⟨ ζ ⟩⟩ {{ Φ }}.
   Proof.
     iIntros "H P /=". simpl_eval.
     iApply (imp_bind _ _ (λ v, ret (VData c v)) with "[H]").
@@ -284,7 +284,7 @@ Section imp_rules_expr.
   Lemma imp_EConstant `{Encode A} {Φ : A → iProp Σ} {ζ} (a : A) η c :
     #a = VConstant c →
     Φ a -∗
-    imp^{ι} eval η (EConstant c) @ E <|Ψ|> ⟨⟨ ζ ⟩⟩ {{ Φ }}.
+    imp eval η (EConstant c) @ E <|Ψ|> ⟨⟨ ζ ⟩⟩ {{ Φ }}.
   Proof.
     iIntros (Henc) "H". simpl_eval.
     by iApply imp_ret.
@@ -294,10 +294,10 @@ Section imp_rules_expr.
   Lemma imp_EXData `{Encode A} {ζ} η π l es (Φs : list (val → iProp Σ)) (Φ : A → iProp Σ) :
     lookup_path η π = ret (VLoc l) →
     ([∗ list] ei;Φi ∈ es;Φs,
-       imp^{ι} eval η ei @ E <|Ψ|> ⟨⟨ ζ ⟩⟩ {{ Φi }}) -∗
+       imp eval η ei @ E <|Ψ|> ⟨⟨ ζ ⟩⟩ {{ Φi }}) -∗
     (∀ vs, ([∗ list] vi;Φi ∈ vs;Φs, Φi vi) -∗
            ∃ (a : A), ⌜#a = VXData l vs⌝ ∗ Φ a) -∗
-    imp^{ι} eval η (EXData π es) @ E <|Ψ|> ⟨⟨ ζ ⟩⟩ {{ Φ }}.
+    imp eval η (EXData π es) @ E <|Ψ|> ⟨⟨ ζ ⟩⟩ {{ Φ }}.
   Proof.
     iIntros (Hlookup) "He Hjoin".
     simpl_eval. rewrite Hlookup. simpl.
@@ -320,7 +320,7 @@ Section imp_rules_expr.
   (** * EInt : Z → expr *)
 
   Lemma imp_EInt {ζ} η i :
-    ⊢ imp^{ι} eval η (EInt i) @ E <|Ψ|> ⟨⟨ ζ ⟩⟩ {{ λ n, ⌜n = i⌝ }}.
+    ⊢ imp eval η (EInt i) @ E <|Ψ|> ⟨⟨ ζ ⟩⟩ {{ λ n, ⌜n = i⌝ }}.
   Proof.
     simpl_eval; by iApply imp_ret.
   Qed.
@@ -331,12 +331,12 @@ Section imp_rules_expr.
   (** * EIntAdd : expr → expr → expr *)
 
   Lemma imp_EIntAdd2 {ζ ζ1 ζ2} η e1 e2 (Φ1 Φ2 : Z → iProp Σ) Φ :
-    imp^{ι} eval η e1 @ E <|Ψ|> ⟨⟨ ζ1 ⟩⟩ {{ Φ1 }} -∗
-    imp^{ι} eval η e2 @ E <|Ψ|> ⟨⟨ ζ2 ⟩⟩ {{ Φ2 }} -∗
+    imp eval η e1 @ E <|Ψ|> ⟨⟨ ζ1 ⟩⟩ {{ Φ1 }} -∗
+    imp eval η e2 @ E <|Ψ|> ⟨⟨ ζ2 ⟩⟩ {{ Φ2 }} -∗
     ▷ (∀ e, ζ1 e -∗ ζ e) ∧
     ▷ (∀ e, ζ2 e -∗ ζ e) ∧
     ▷ (∀ i j, Φ1 i -∗ Φ2 j -∗ Φ (i + j)) -∗
-    imp^{ι} eval η (EIntAdd e1 e2) @ E <|Ψ|> ⟨⟨ ζ ⟩⟩ {{ Φ }}.
+    imp eval η (EIntAdd e1 e2) @ E <|Ψ|> ⟨⟨ ζ ⟩⟩ {{ Φ }}.
   Proof.
     iIntros "H1 H2 Hjoin /=". simpl_eval.
     iApply (imp_Par _ ζ1 _ ζ2 (as_int (eval η e1)) (as_int (eval η e2)) with "[H1] [H2]").
@@ -367,10 +367,10 @@ Section imp_rules_expr.
   Qed.
 
   Lemma imp_EIntAdd {ζ Φ} η e1 e2 (Φ1 Φ2 : Z → iProp Σ) :
-    imp^{ι} eval η e1 @ E <|Ψ|> ⟨⟨ ζ ⟩⟩ {{ Φ1 }} -∗
-    imp^{ι} eval η e2 @ E <|Ψ|> ⟨⟨ ζ ⟩⟩ {{ Φ2 }} -∗
+    imp eval η e1 @ E <|Ψ|> ⟨⟨ ζ ⟩⟩ {{ Φ1 }} -∗
+    imp eval η e2 @ E <|Ψ|> ⟨⟨ ζ ⟩⟩ {{ Φ2 }} -∗
     ▷ (∀ i j, Φ1 i -∗ Φ2 j -∗ Φ (i + j)%Z) -∗
-    imp^{ι} eval η (EIntAdd e1 e2) @ E <|Ψ|> ⟨⟨ ζ ⟩⟩ {{ Φ }}.
+    imp eval η (EIntAdd e1 e2) @ E <|Ψ|> ⟨⟨ ζ ⟩⟩ {{ Φ }}.
   Proof.
     iIntros "H1 H2 P".
     iApply (imp_EIntAdd2 with "H1 H2").
@@ -397,13 +397,13 @@ Section imp_rules_expr.
   Local Instance observe_bool : Observe bool bool := { observe := id }.
 
   Lemma imp_EOpEq2 {Φ : bool → iProp Σ} {ζ ζ1 ζ2} η e1 e2 Φ1 Φ2 :
-    imp^{ι} eval η e1 @ E <|Ψ|> ⟨⟨ ζ1 ⟩⟩ {{ Φ1 }} -∗
-    imp^{ι} eval η e2 @ E <|Ψ|> ⟨⟨ ζ2 ⟩⟩ {{ Φ2 }} -∗
+    imp eval η e1 @ E <|Ψ|> ⟨⟨ ζ1 ⟩⟩ {{ Φ1 }} -∗
+    imp eval η e2 @ E <|Ψ|> ⟨⟨ ζ2 ⟩⟩ {{ Φ2 }} -∗
     ▷ (∀ e, ζ1 e -∗ ζ e) ∧
     ▷ (∀ e, ζ2 e -∗ ζ e) ∧
     ▷ (∀ v1 v2, Φ1 v1 -∗ Φ2 v2 -∗
-              imp^{ι} eq_val v1 v2 @ E <|Ψ|> ⟨⟨ ζ ⟩⟩ {{ Φ }}) -∗
-    imp^{ι} eval η (EOpEq e1 e2) @ E <|Ψ|> ⟨⟨ ζ ⟩⟩ {{ Φ }}.
+              imp eq_val v1 v2 @ E <|Ψ|> ⟨⟨ ζ ⟩⟩ {{ Φ }}) -∗
+    imp eval η (EOpEq e1 e2) @ E <|Ψ|> ⟨⟨ ζ ⟩⟩ {{ Φ }}.
   Proof.
     iIntros "H1 H2 Hjoin". simpl_eval.
     iApply (imp_Par _ _ _ _ _ _
@@ -426,12 +426,12 @@ Section imp_rules_expr.
   Qed.
 
   Lemma imp_EOpEq  {Φ : bool → iProp Σ} {ζ} η e1 e2 Φ1 Φ2 :
-    imp^{ι} eval η e1 @ E <|Ψ|> ⟨⟨ ζ ⟩⟩ {{ Φ1 }} -∗
-    imp^{ι} eval η e2 @ E <|Ψ|> ⟨⟨ ζ ⟩⟩ {{ Φ2 }} -∗
+    imp eval η e1 @ E <|Ψ|> ⟨⟨ ζ ⟩⟩ {{ Φ1 }} -∗
+    imp eval η e2 @ E <|Ψ|> ⟨⟨ ζ ⟩⟩ {{ Φ2 }} -∗
     ▷ (∀ v1 v2,
          Φ1 v1 -∗ Φ2 v2 -∗
-         imp^{ι} eq_val v1 v2 @ E <|Ψ|> ⟨⟨ ζ ⟩⟩ {{ Φ }}) -∗
-    imp^{ι} eval η (EOpEq e1 e2) @ E <|Ψ|> ⟨⟨ ζ ⟩⟩ {{ Φ }}.
+         imp eq_val v1 v2 @ E <|Ψ|> ⟨⟨ ζ ⟩⟩ {{ Φ }}) -∗
+    imp eval η (EOpEq e1 e2) @ E <|Ψ|> ⟨⟨ ζ ⟩⟩ {{ Φ }}.
   Proof.
     iIntros "H1 H2 P".
     iApply (imp_EOpEq2 with "H1 H2"); auto.
@@ -440,9 +440,9 @@ Section imp_rules_expr.
   Lemma imp_EOpEq_Z {ζ} η e1 e2 (i j : Z) :
     representable i ->
     representable j ->
-    imp^{ι} eval η e1 @ E <|Ψ|> ⟨⟨ ζ ⟩⟩ {{ λ n, ⌜n = i⌝ }} -∗
-    imp^{ι} eval η e2 @ E <|Ψ|> ⟨⟨ ζ ⟩⟩ {{ λ n, ⌜n = j⌝ }} -∗
-    imp^{ι} eval η (EOpEq e1 e2) @ E <|Ψ|> ⟨⟨ ζ ⟩⟩ {{ λ b, ⌜b = (i =? j)%Z⌝ }}.
+    imp eval η e1 @ E <|Ψ|> ⟨⟨ ζ ⟩⟩ {{ λ n, ⌜n = i⌝ }} -∗
+    imp eval η e2 @ E <|Ψ|> ⟨⟨ ζ ⟩⟩ {{ λ n, ⌜n = j⌝ }} -∗
+    imp eval η (EOpEq e1 e2) @ E <|Ψ|> ⟨⟨ ζ ⟩⟩ {{ λ b, ⌜b = (i =? j)%Z⌝ }}.
   Proof.
     iIntros (Hn1 Hn2) "H1 H2".
     iApply (imp_EOpEq with "[H1] [H2]").
@@ -473,9 +473,9 @@ Section imp_rules_expr.
 
   (* Intermediate lemma: using [eval_bindings] hypothesis *)
   Lemma imp_ELet `{Encode A} {Φ : A → iProp Σ} {ζ} η bs e Φ1 :
-    imp^{ι} eval_bindings η bs @ E <|Ψ|> ⟨⟨ ζ ⟩⟩ {{ Φ1 }} -∗
-    (∀ (δ : env), Φ1 δ -∗ imp^{ι} eval (δ ++ η) e @ E <|Ψ|> ⟨⟨ ζ ⟩⟩ {{ Φ }}) -∗
-    imp^{ι} eval η (ELet bs e) @ E <|Ψ|> ⟨⟨ ζ ⟩⟩ {{ Φ }}.
+    imp eval_bindings η bs @ E <|Ψ|> ⟨⟨ ζ ⟩⟩ {{ Φ1 }} -∗
+    (∀ (δ : env), Φ1 δ -∗ imp eval (δ ++ η) e @ E <|Ψ|> ⟨⟨ ζ ⟩⟩ {{ Φ }}) -∗
+    imp eval η (ELet bs e) @ E <|Ψ|> ⟨⟨ ζ ⟩⟩ {{ Φ }}.
   Proof.
     iIntros "Hbindings P /=". simpl_eval.
     iApply (imp_bind _ _ (λ (δ : env), eval (δ ++ η) e) with "Hbindings").
@@ -485,11 +485,11 @@ Section imp_rules_expr.
 
   Local Lemma imp_bindings_cons `{Encode A} {Φ Φ' : env → iProp Σ} {ζ} (Φ1 : A → iProp Σ)
     η p e bs (φs : val -> env -> Prop) :
-    imp^{ι} eval η e @ E <|Ψ|> ⟨⟨ ζ ⟩⟩ {{ Φ1 }} -∗
-    imp^{ι} eval_bindings η bs @ E <|Ψ|> ⟨⟨ ζ ⟩⟩ {{ Φ' }} -∗
+    imp eval η e @ E <|Ψ|> ⟨⟨ ζ ⟩⟩ {{ Φ1 }} -∗
+    imp eval_bindings η bs @ E <|Ψ|> ⟨⟨ ζ ⟩⟩ {{ Φ' }} -∗
     (∀ x δ, Φ1 x -∗ Φ' δ -∗ ⌜pattern η δ p #x (φs #x) False⌝) -∗
     (∀ x δ, Φ1 x -∗  ⌜φs #x δ⌝ -∗ Φ δ) -∗
-    imp^{ι} eval_bindings η (Binding p e :: bs) @ E <|Ψ|> ⟨⟨ ζ ⟩⟩ {{ Φ }}.
+    imp eval_bindings η (Binding p e :: bs) @ E <|Ψ|> ⟨⟨ ζ ⟩⟩ {{ Φ }}.
   Proof.
     iIntros "H1 H2 P Hcons /=".
     simpl_eval_bindings.
@@ -518,10 +518,10 @@ Section imp_rules_expr.
   Qed.
 
   Lemma imp_bindings_singleton `{Encode A} {ζ} {Φ : env → iProp Σ} (Φ1 : A → iProp Σ) {η p e} φs :
-    imp^{ι} eval η e @ E <|Ψ|> ⟨⟨ ζ ⟩⟩ {{ Φ1 }} -∗
+    imp eval η e @ E <|Ψ|> ⟨⟨ ζ ⟩⟩ {{ Φ1 }} -∗
     (∀ x, Φ1 x -∗ ⌜pattern η nil p #x (φs #x) False⌝) -∗
     (∀ x δ, Φ1 x -∗ ⌜φs #x δ⌝ -∗ Φ δ) -∗
-    imp^{ι} eval_bindings η [ Binding p e ] @ E <|Ψ|> ⟨⟨ ζ ⟩⟩ {{ Φ }}.
+    imp eval_bindings η [ Binding p e ] @ E <|Ψ|> ⟨⟨ ζ ⟩⟩ {{ Φ }}.
   Proof.
     iIntros "H1 P /=".
     iApply (imp_bindings_cons with "H1").
@@ -534,11 +534,11 @@ Section imp_rules_expr.
 
   (* TODO: Have *_singleton *_cons lemmas about relevant expr constructs *)
   Corollary imp_ELet_singleton `{Encode A, Encode B} {Φ : A → iProp Σ} {ζ} {Φ1 : B → iProp Σ} {η p e e'} φ :
-    imp^{ι} eval η e' @ E <|Ψ|> ⟨⟨ ζ ⟩⟩ {{ Φ1 }} -∗
+    imp eval η e' @ E <|Ψ|> ⟨⟨ ζ ⟩⟩ {{ Φ1 }} -∗
     (∀ (x : B), Φ1 x -∗ ⌜pattern η nil p (#x) (φ #x) False⌝) -∗
     (∀ x δ, Φ1 x -∗ ⌜φ #x δ⌝ -∗
-            imp^{ι} eval (δ ++ η) e @ E <|Ψ|> ⟨⟨ ζ ⟩⟩ {{ Φ }}) -∗
-    imp^{ι} eval η (ELet [ Binding p e' ] e) @ E <|Ψ|> ⟨⟨ ζ ⟩⟩ {{ Φ }}.
+            imp eval (δ ++ η) e @ E <|Ψ|> ⟨⟨ ζ ⟩⟩ {{ Φ }}) -∗
+    imp eval η (ELet [ Binding p e' ] e) @ E <|Ψ|> ⟨⟨ ζ ⟩⟩ {{ Φ }}.
   Proof.
     iIntros "He' HP He".
     iApply (imp_ELet with "[He' HP He]").
@@ -548,9 +548,9 @@ Section imp_rules_expr.
 
   (* Special case of [let x = e' in e] *)
   Lemma imp_ELet_var `{Encode A, Encode B} {ζ} {Φ : A → iProp Σ} (Φ' : B → iProp Σ) {η x e e'} :
-    imp^{ι} eval η e' @ E <|Ψ|> ⟨⟨ ζ ⟩⟩ {{ Φ' }} -∗
-    (∀ b, Φ' b -∗ imp^{ι} eval ((x, #b) :: η) e @ E <|Ψ|> ⟨⟨ ζ ⟩⟩ {{ Φ }}) -∗
-    imp^{ι}eval η (ELet [Binding (PVar x) e'] e) @ E <|Ψ|> ⟨⟨ ζ ⟩⟩ {{ Φ }}.
+    imp eval η e' @ E <|Ψ|> ⟨⟨ ζ ⟩⟩ {{ Φ' }} -∗
+    (∀ b, Φ' b -∗ imp eval ((x, #b) :: η) e @ E <|Ψ|> ⟨⟨ ζ ⟩⟩ {{ Φ }}) -∗
+    imp eval η (ELet [Binding (PVar x) e'] e) @ E <|Ψ|> ⟨⟨ ζ ⟩⟩ {{ Φ }}.
   Proof.
     iIntros "H P".
     iApply (imp_ELet_singleton with "H").
@@ -564,9 +564,9 @@ Section imp_rules_expr.
 
   (* Special case of [let _ = e' in e] *)
   Lemma imp_ELet_wild `{Encode A, Encode B} {ζ} {Φ : A → iProp Σ} (R : iProp Σ) {η e e'} :
-    imp^{ι} eval η e' @ E <|Ψ|> ⟨⟨ ζ ⟩⟩ {{ λ (_ : B), R }} -∗
-    (R -∗ imp^{ι} eval η e @ E <|Ψ|> ⟨⟨ ζ ⟩⟩ {{ Φ }}) -∗
-    imp^{ι} eval η (ELet [Binding PAny e'] e) @ E <|Ψ|> ⟨⟨ ζ ⟩⟩ {{ Φ }}.
+    imp eval η e' @ E <|Ψ|> ⟨⟨ ζ ⟩⟩ {{ λ (_ : B), R }} -∗
+    (R -∗ imp eval η e @ E <|Ψ|> ⟨⟨ ζ ⟩⟩ {{ Φ }}) -∗
+    imp eval η (ELet [Binding PAny e'] e) @ E <|Ψ|> ⟨⟨ ζ ⟩⟩ {{ Φ }}.
   Proof.
     iIntros "H P".
     iApply (imp_ELet_singleton with "H").
@@ -580,9 +580,9 @@ Section imp_rules_expr.
 
   (* Special case of [let (x, y) = e' in e] *)
   Lemma imp_ELet_pair `{Encode C, Encode A, Encode B} {ζ} {Φ : C → iProp Σ} (Φ' : A * B → iProp Σ) {η x y e e'} :
-    imp^{ι} eval η e' @ E <|Ψ|> ⟨⟨ ζ ⟩⟩ {{ Φ' }} -∗
-    (∀ a b, Φ' (a, b) -∗ imp^{ι} eval ((y, #b) :: (x, #a) :: η) e @ E <|Ψ|> ⟨⟨ ζ ⟩⟩ {{ Φ }}) -∗
-    imp^{ι} eval η (ELet [Binding (PTuple [PVar x; PVar y]) e'] e) @ E <|Ψ|> ⟨⟨ ζ ⟩⟩ {{ Φ }}.
+    imp eval η e' @ E <|Ψ|> ⟨⟨ ζ ⟩⟩ {{ Φ' }} -∗
+    (∀ a b, Φ' (a, b) -∗ imp eval ((y, #b) :: (x, #a) :: η) e @ E <|Ψ|> ⟨⟨ ζ ⟩⟩ {{ Φ }}) -∗
+    imp eval η (ELet [Binding (PTuple [PVar x; PVar y]) e'] e) @ E <|Ψ|> ⟨⟨ ζ ⟩⟩ {{ Φ }}.
   Proof.
     iIntros "H P".
     iApply (imp_ELet_singleton with "H").
@@ -601,8 +601,8 @@ Section imp_rules_expr.
 
   Lemma imp_ELetRec `{Encode A} {Φ : A → iProp Σ} {ζ} η bs e :
     let δ := eval_rec_bindings η bs in
-    imp^{ι} eval (δ ++ η) e @ E <|Ψ|> ⟨⟨ ζ ⟩⟩ {{ Φ }} -∗
-    imp^{ι} eval η (ELetRec bs e) @ E <|Ψ|> ⟨⟨ ζ ⟩⟩ {{ Φ }}.
+    imp eval (δ ++ η) e @ E <|Ψ|> ⟨⟨ ζ ⟩⟩ {{ Φ }} -∗
+    imp eval η (ELetRec bs e) @ E <|Ψ|> ⟨⟨ ζ ⟩⟩ {{ Φ }}.
   Proof.
     simpl_eval; auto.
   Qed.
@@ -611,9 +611,9 @@ Section imp_rules_expr.
 
   (** * ELetOpen : mexpr → expr → expr *)
   Lemma imp_ELetOpen `{Encode A} {Φ : A → iProp Σ} {ζ} (Φ' : env → iProp Σ) η me e :
-    imp^{ι} eval_mexpr η me @ E <|Ψ|> ⟨⟨ ζ ⟩⟩ {{ Φ' }} -∗
-    (∀ δ, Φ' δ -∗ imp^{ι} eval (δ ++ η) e @ E <|Ψ|> ⟨⟨ ζ ⟩⟩ {{ Φ }}) -∗
-    imp^{ι} eval η (ELetOpen me e) @ E <|Ψ|> ⟨⟨ ζ ⟩⟩ {{ Φ }}.
+    imp eval_mexpr η me @ E <|Ψ|> ⟨⟨ ζ ⟩⟩ {{ Φ' }} -∗
+    (∀ δ, Φ' δ -∗ imp eval (δ ++ η) e @ E <|Ψ|> ⟨⟨ ζ ⟩⟩ {{ Φ }}) -∗
+    imp eval η (ELetOpen me e) @ E <|Ψ|> ⟨⟨ ζ ⟩⟩ {{ Φ }}.
   Proof.
     iIntros "Hme He". simpl_eval.
     iApply (imp_bind _ _ (λ δ, eval (δ ++ η) e) with "[Hme]").
@@ -628,9 +628,9 @@ Section imp_rules_expr.
   (** * ESeq : expr → expr → expr *)
 
   Lemma imp_ESeq `{Encode A, Encode B} {Φ : A → iProp Σ} {ζ} (Φ1 : B → iProp Σ) η e1 e2 :
-    imp^{ι} eval η e1 @ E <|Ψ|> ⟨⟨ ζ ⟩⟩ {{ Φ1 }} -∗
-    (∀ x, Φ1 x -∗ imp^{ι} eval η e2 @ E <|Ψ|> ⟨⟨ ζ ⟩⟩ {{ Φ }}) -∗
-    imp^{ι}eval η (ESeq e1 e2) @ E <|Ψ|> ⟨⟨ ζ ⟩⟩ {{ Φ }}.
+    imp eval η e1 @ E <|Ψ|> ⟨⟨ ζ ⟩⟩ {{ Φ1 }} -∗
+    (∀ x, Φ1 x -∗ imp eval η e2 @ E <|Ψ|> ⟨⟨ ζ ⟩⟩ {{ Φ }}) -∗
+    imp eval η (ESeq e1 e2) @ E <|Ψ|> ⟨⟨ ζ ⟩⟩ {{ Φ }}.
   Proof.
     iIntros "He1 He2 /=". simpl_eval.
     iApply (imp_bind _ _ (λ (_ : val), eval η e2) with "He1 He2").
@@ -639,11 +639,11 @@ Section imp_rules_expr.
   (** * EIfThen : expr → expr → expr *)
 
   Lemma imp_EIfThen {Φ : unit → iProp Σ} {ζ} η eb e1 (Φb : bool → iProp Σ) :
-    imp^{ι} eval η eb @ E <|Ψ|> ⟨⟨ ζ ⟩⟩ {{ Φb }} -∗
+    imp eval η eb @ E <|Ψ|> ⟨⟨ ζ ⟩⟩ {{ Φb }} -∗
     (∀ b, Φb b -∗
-          if b then imp^{ι} eval η e1 @ E <|Ψ|> ⟨⟨ ζ ⟩⟩ {{ Φ }}
+          if b then imp eval η e1 @ E <|Ψ|> ⟨⟨ ζ ⟩⟩ {{ Φ }}
           else Φ ()) -∗
-    imp^{ι} eval η (EIfThen eb e1) @ E <|Ψ|> ⟨⟨ ζ ⟩⟩ {{ Φ }}.
+    imp eval η (EIfThen eb e1) @ E <|Ψ|> ⟨⟨ ζ ⟩⟩ {{ Φ }}.
   Proof.
     iIntros "Hb He /=". simpl_eval.
     iApply (imp_bind _ _ (λ (b : bool), if b then eval η e1 else ret VUnit) with "[Hb]").
@@ -662,11 +662,11 @@ Section imp_rules_expr.
   (** * EIfThenElse : expr → expr → expr → expr *)
 
   Lemma imp_EIfThenElse `{Encode A} {Φ : A → iProp Σ} {ζ} η eb e1 e2 (Φb : bool → iProp Σ) :
-    imp^{ι} eval η eb @ E <|Ψ|> ⟨⟨ ζ ⟩⟩ {{ Φb }} -∗
+    imp eval η eb @ E <|Ψ|> ⟨⟨ ζ ⟩⟩ {{ Φb }} -∗
     (∀ b, Φb b -∗
-          if b then imp^{ι} eval η e1 @ E <|Ψ|> ⟨⟨ ζ ⟩⟩ {{ Φ }}
-          else imp^{ι} eval η e2 @ E <|Ψ|> ⟨⟨ ζ ⟩⟩ {{ Φ }}) -∗
-    imp^{ι} eval η (EIfThenElse eb e1 e2) @ E <|Ψ|> ⟨⟨ ζ ⟩⟩ {{ Φ }}.
+          if b then imp eval η e1 @ E <|Ψ|> ⟨⟨ ζ ⟩⟩ {{ Φ }}
+          else imp eval η e2 @ E <|Ψ|> ⟨⟨ ζ ⟩⟩ {{ Φ }}) -∗
+    imp eval η (EIfThenElse eb e1 e2) @ E <|Ψ|> ⟨⟨ ζ ⟩⟩ {{ Φ }}.
   Proof.
     iIntros "Hb He /=". simpl_eval.
     iApply (imp_bind _ _ (λ (b : bool), if b then eval η e1 else eval η e2) with "[Hb]").
@@ -683,8 +683,8 @@ Section imp_rules_expr.
   (** * EMatch : expr → list branch → expr *)
 
   Lemma imp_EMatch `{Encode A} {Φ : A → iProp Σ} {ζ} η e bs :
-    imp^{ι} deep_handler η e bs @ E <|Ψ|> ⟨⟨ ζ ⟩⟩ {{ Φ }} -∗
-    imp^{ι} eval η (EMatch e bs) @ E <|Ψ|> ⟨⟨ ζ ⟩⟩ {{ Φ }}.
+    imp deep_handler η e bs @ E <|Ψ|> ⟨⟨ ζ ⟩⟩ {{ Φ }} -∗
+    imp eval η (EMatch e bs) @ E <|Ψ|> ⟨⟨ ζ ⟩⟩ {{ Φ }}.
   Proof.
     by iIntros "H"; simpl_eval.
   Qed.
@@ -692,12 +692,12 @@ Section imp_rules_expr.
   (** * ERaise : expr → expr *)
 
   Lemma imp_ERaise `{Encode A} {Φ : A → iProp Σ} {ζ} η e :
-    imp^{ι} eval η e @ E <|Ψ|> ⟨⟨ ζ ⟩⟩ {{ ζ }} -∗
-    imp^{ι} eval η (ERaise e) @ E <|Ψ|> ⟨⟨ ζ ⟩⟩ {{ Φ }}.
+    imp eval η e @ E <|Ψ|> ⟨⟨ ζ ⟩⟩ {{ ζ }} -∗
+    imp eval η (ERaise e) @ E <|Ψ|> ⟨⟨ ζ ⟩⟩ {{ Φ }}.
   Proof.
     iIntros "H". simpl_eval.
     iApply (@imp_bind _ _ A val exn _ _
-              ι E Ψ ζ Φ
+              E Ψ ζ Φ
               val _ val _ ζ (eval η e) (λ v, throw v) with "H").
     iIntros (ex) "Hζ". change (♯ex) with ex.
     iApply (@imp_throw _ _ A val exn with "Hζ").
@@ -710,8 +710,8 @@ Section imp_rules_expr.
   (** * EAssert : expr → expr *)
 
   Lemma imp_EAssert {R : iProp Σ} {ζ} η e :
-    R ∧ imp^{ι} eval η e @ E <|Ψ|> ⟨⟨ ζ ⟩⟩ {{ λ b, ⌜b = true⌝ ∗ R }} -∗
-    imp^{ι} eval η (EAssert e) @ E <|Ψ|> ⟨⟨ ζ ⟩⟩ {{ λ (_ : unit), R }}.
+    R ∧ imp eval η e @ E <|Ψ|> ⟨⟨ ζ ⟩⟩ {{ λ b, ⌜b = true⌝ ∗ R }} -∗
+    imp eval η (EAssert e) @ E <|Ψ|> ⟨⟨ ζ ⟩⟩ {{ λ (_ : unit), R }}.
   Proof.
     iIntros "H /=". simpl_eval.
     iApply (imp_choose
@@ -736,9 +736,9 @@ Section imp_rules_expr.
 
   (** * ERef : expr → expr *)
 
-  Lemma imp_ERef `{Encode A} {ζ} (Φ : A → iProp Σ) η e :
-    imp^{ι} eval η e @ E <|Ψ|> ⟨⟨ ζ ⟩⟩ {{ Φ }} -∗
-    imp^{ι} eval η (ERef e) @ E <|Ψ|> ⟨⟨ ζ ⟩⟩ {{ λ l, ∃ a, Φ a ∗ l ↦ (V #a) }}.
+  Lemma imp_ERef2 `{Encode A} {ζ} (Φ : A → iProp Σ) η e :
+    imp eval η e @ E <|Ψ|> ⟨⟨ ζ ⟩⟩ {{ Φ }} -∗
+    imp eval η (ERef e) @ E <|Ψ|> ⟨⟨ ζ ⟩⟩ {{ λ l, ∃ a, Φ a ∗ l ↦ (V #a) }}.
   Proof.
     iIntros "He". simpl_eval.
     iApply (imp_bind _ _
@@ -756,12 +756,22 @@ Section imp_rules_expr.
     iFrame.
   Qed.
 
+  Lemma imp_ERef `{Encode A} {ζ} (a : A) η e :
+    imp eval η e @ E <|Ψ|> ⟨⟨ ζ ⟩⟩ {{ λ a', ⌜a' = a⌝ }} -∗
+    imp eval η (ERef e) @ E <|Ψ|> ⟨⟨ ζ ⟩⟩ {{ λ l, l ↦ (V #a) }}.
+  Proof.
+    iIntros "He".
+    iApply (imp_mono_ret (λ l, ∃ a', ⌜a' = a⌝ ∗ l ↦ (V #a'))%I with "[He]").
+    iApply (imp_ERef2 with "He").
+    iIntros (l) "(% & -> & $)".
+  Qed.
+
   (** * ELoad : expr → expr *)
 
   Lemma imp_ELoad2 `{Encode A} {Φ : A → iProp Σ} {ζ} (Φ1 : loc → iProp Σ) η e :
-    imp^{ι} (eval η e) @ E <|Ψ|> ⟨⟨ ζ ⟩⟩ {{ Φ1 }} -∗
+    imp (eval η e) @ E <|Ψ|> ⟨⟨ ζ ⟩⟩ {{ Φ1 }} -∗
     (∀ l, Φ1 l -∗ ∃ q a, ▷ pointsto l q (V #a) ∗ ▷ (pointsto l q (V #a) -∗ Φ a)) -∗
-    imp^{ι} eval η (ELoad e) @ E <|Ψ|> ⟨⟨ ζ ⟩⟩ {{ Φ }}.
+    imp eval η (ELoad e) @ E <|Ψ|> ⟨⟨ ζ ⟩⟩ {{ Φ }}.
   Proof.
     iIntros "He P". simpl_eval.
     iApply (imp_bind _ _ (λ l, load l) with "[He]").
@@ -782,8 +792,8 @@ Section imp_rules_expr.
 
   Lemma imp_ELoad `{Encode A} {Φ : A → iProp Σ} {ζ} η e l q (a : A) :
     ▷ pointsto l q (V #a) -∗
-    imp^{ι} eval η e @ E <|Ψ|> ⟨⟨ ζ ⟩⟩ {{ λ l', ⌜l' = l⌝ }} -∗
-    imp^{ι} eval η (ELoad e) @ E <|Ψ|> ⟨⟨ ζ ⟩⟩ {{ λ v, ⌜v = a⌝ ∗ pointsto l q (V #a) }}.
+    imp eval η e @ E <|Ψ|> ⟨⟨ ζ ⟩⟩ {{ λ l', ⌜l' = l⌝ }} -∗
+    imp eval η (ELoad e) @ E <|Ψ|> ⟨⟨ ζ ⟩⟩ {{ λ v, ⌜v = a⌝ ∗ pointsto l q (V #a) }}.
   Proof.
     iIntros "Hl He /=".
     iApply (imp_ELoad2 with "He").
@@ -794,11 +804,11 @@ Section imp_rules_expr.
   (** * EStore : expr → expr → expr *)
 
   Lemma imp_EStore2 `{Encode A} {Φ : unit → iProp Σ} {ζ} η e1 e2 (Φ1 : loc → iProp Σ) (Φ2 : A → iProp Σ) :
-    imp^{ι} eval η e1 @ E <|Ψ|> ⟨⟨ ζ ⟩⟩ {{ Φ1 }} -∗
-    imp^{ι} eval η e2 @ E <|Ψ|> ⟨⟨ ζ ⟩⟩ {{ Φ2 }} -∗
+    imp eval η e1 @ E <|Ψ|> ⟨⟨ ζ ⟩⟩ {{ Φ1 }} -∗
+    imp eval η e2 @ E <|Ψ|> ⟨⟨ ζ ⟩⟩ {{ Φ2 }} -∗
     (∀ l a, Φ1 l -∗ Φ2 a -∗
       ▷ ∃ v1, l ↦ (V v1) ∗ ▷ (l ↦ (V #a) -∗ Φ ())) -∗
-    imp^{ι} eval η (EStore e1 e2) @ E <|Ψ|> ⟨⟨ ζ ⟩⟩ {{ Φ }}.
+    imp eval η (EStore e1 e2) @ E <|Ψ|> ⟨⟨ ζ ⟩⟩ {{ Φ }}.
   Proof.
     iIntros "H1 H2 P /=". simpl_eval.
     iApply (imp_Par _ _ _ _ _ _
@@ -825,9 +835,9 @@ Section imp_rules_expr.
 
   Lemma imp_EStore `{Encode A} {ζ} (Φ : A → iProp Σ) {η e1 e2} l v :
     ▷ l ↦ (V v) -∗
-    imp^{ι} eval η e1 @ E <|Ψ|> ⟨⟨ ζ ⟩⟩ {{ λ l', ⌜l' = l⌝ }} -∗
-    imp^{ι} eval η e2 @ E <|Ψ|> ⟨⟨ ζ ⟩⟩ {{ Φ }} -∗
-    imp^{ι} eval η (EStore e1 e2) @ E <|Ψ|> ⟨⟨ ζ ⟩⟩ {{ λ (_ : unit), ∃ a, l ↦ (V #a) ∗ Φ a }}.
+    imp eval η e1 @ E <|Ψ|> ⟨⟨ ζ ⟩⟩ {{ λ l', ⌜l' = l⌝ }} -∗
+    imp eval η e2 @ E <|Ψ|> ⟨⟨ ζ ⟩⟩ {{ Φ }} -∗
+    imp eval η (EStore e1 e2) @ E <|Ψ|> ⟨⟨ ζ ⟩⟩ {{ λ (_ : unit), ∃ a, l ↦ (V #a) ∗ Φ a }}.
   Proof.
     iIntros "Hl H1 H2".
     iApply (imp_EStore2 with "H1 H2").
@@ -839,9 +849,9 @@ Section imp_rules_expr.
   (** * EPerform : expr -> expr *)
 
   Lemma imp_EPerform `{Encode A, Encode B} {Φ : A → iProp Σ} {ζ} (Φ1 : B → iProp Σ) η e :
-    imp^{ι} eval η e @ E <|Ψ|> ⟨⟨ ζ ⟩⟩ {{ Φ1 }} -∗
+    imp eval η e @ E <|Ψ|> ⟨⟨ ζ ⟩⟩ {{ Φ1 }} -∗
     (∀ x, Φ1 x -∗ Ψ allows perform #x << ilift ζ (ireturns Φ) >>) -∗
-    imp^{ι} eval η (EPerform e) @ E <|Ψ|> ⟨⟨ ζ ⟩⟩ {{ Φ }}.
+    imp eval η (EPerform e) @ E <|Ψ|> ⟨⟨ ζ ⟩⟩ {{ Φ }}.
   Proof.
     iIntros "He Hv". simpl_eval.
     iApply (imp_bind _ _ (λ eff, perform eff) with "He").
@@ -854,11 +864,11 @@ Section imp_rules_expr.
 
   Local Lemma imp_EContinue' `{Encode A, Encode B} {Φ : A → iProp Σ} {ζ}
     η e1 e2 (Φ1 : cont → iProp Σ) (Φ2 : B → iProp Σ) :
-    imp^{ι} eval η e1 @ E <|Ψ|> ⟨⟨ ζ ⟩⟩ {{ Φ1 }} -∗
-    imp^{ι} eval η e2 @ E <|Ψ|> ⟨⟨ ζ ⟩⟩ {{ Φ2 }} -∗
+    imp eval η e1 @ E <|Ψ|> ⟨⟨ ζ ⟩⟩ {{ Φ1 }} -∗
+    imp eval η e2 @ E <|Ψ|> ⟨⟨ ζ ⟩⟩ {{ Φ2 }} -∗
     (∀ (k : cont) x, Φ1 k -∗ Φ2 x -∗
-                ▷ imp^{ι} stop CResume (k, O2Ret #x) @ E <|Ψ|> ⟨⟨ ζ ⟩⟩ {{ Φ }}) -∗
-    imp^{ι} eval η (EContinue e1 e2) @ E <|Ψ|> ⟨⟨ ζ ⟩⟩ {{ Φ }}.
+                ▷ imp stop CResume (k, O2Ret #x) @ E <|Ψ|> ⟨⟨ ζ ⟩⟩ {{ Φ }}) -∗
+    imp eval η (EContinue e1 e2) @ E <|Ψ|> ⟨⟨ ζ ⟩⟩ {{ Φ }}.
   Proof.
     iIntros "Hk Hv Hmon". simpl_eval.
     iApply (imp_Par _ _ _ _ _ _ (pfbind inject2 (λ '(l, v), resume l (O2Ret v))) with "[Hk] Hv [Hmon]").
@@ -880,13 +890,13 @@ Section imp_rules_expr.
 
   Lemma imp_EContinue `{Encode A, Encode B} {Φ : A → iProp Σ} {ζ}
     η e1 e2 (Φ1 : cont → iProp Σ) (Φ2 : B → iProp Σ) :
-    imp^{ι} eval η e1 @ E <|Ψ|> ⟨⟨ ζ ⟩⟩ {{ Φ1 }} -∗
-    imp^{ι} eval η e2 @ E <|Ψ|> ⟨⟨ ζ ⟩⟩ {{ Φ2 }} -∗
+    imp eval η e1 @ E <|Ψ|> ⟨⟨ ζ ⟩⟩ {{ Φ1 }} -∗
+    imp eval η e2 @ E <|Ψ|> ⟨⟨ ζ ⟩⟩ {{ Φ2 }} -∗
     (∀ k x, Φ1 k -∗ Φ2 x -∗
             ∃ sk, isCont k sk ∗
                   ▷ (isShot k -∗
-                     ▷ imp^{ι} (sk (O2Ret #x)) @ E <|Ψ|> ⟨⟨ ζ ⟩⟩ {{ Φ }})) -∗
-    imp^{ι} eval η (EContinue e1 e2) @ E <|Ψ|> ⟨⟨ ζ ⟩⟩ {{ Φ }}.
+                     ▷ imp (sk (O2Ret #x)) @ E <|Ψ|> ⟨⟨ ζ ⟩⟩ {{ Φ }})) -∗
+    imp eval η (EContinue e1 e2) @ E <|Ψ|> ⟨⟨ ζ ⟩⟩ {{ Φ }}.
   Proof.
     iIntros "H1 H2 H3".
     iApply (imp_EContinue' with "H1 H2").
@@ -902,11 +912,11 @@ Section imp_rules_expr.
 
   Local Lemma imp_EFork' `{Encode A, Encode B} {ζ}
     (Φ1 : val → iProp Σ) (Φ2 : B → iProp Σ) μ (φ : A → iProp Σ) η e1 e2 :
-    imp^{ι} eval η e1 @ E <|Ψ|> ⟨⟨ ζ ⟩⟩ {{ Φ1 }} -∗
-    imp^{ι} eval η e2 @ E <|Ψ|> ⟨⟨ ζ ⟩⟩ {{ Φ2 }} -∗
+    imp eval η e1 @ E <|Ψ|> ⟨⟨ ζ ⟩⟩ {{ Φ1 }} -∗
+    imp eval η e2 @ E <|Ψ|> ⟨⟨ ζ ⟩⟩ {{ Φ2 }} -∗
     ▷ (∀ ι' f x, isThread ι' μ φ -∗ Φ1 f -∗ Φ2 x -∗
-                  imp^{ι'} call f #x @ E <| ⊥ |> ⟨⟨ λ e, □ μ e ⟩⟩ {{ λ x, □ φ x }}) -∗
-    imp^{ι} eval η (EFork e1 e2) @ E <|Ψ|> ⟨⟨ ζ ⟩⟩ {{ λ ι, isThread ι μ φ }}.
+                  imp call f #x @ E <| ⊥ |> ⟨⟨ λ e, □ μ e ⟩⟩ {{ λ x, □ φ x }}) -∗
+    imp eval η (EFork e1 e2) @ E <|Ψ|> ⟨⟨ ζ ⟩⟩ {{ λ ι, isThread ι μ φ }}.
   Proof.
     iIntros "H1 H2 Hcall". simpl_eval.
     iApply (imp_Par _ _ _ _ _ _ (pfbind inject2 (λ '(f, v), fork f v)) with "H1 H2").
@@ -924,11 +934,11 @@ Section imp_rules_expr.
 
   Lemma imp_EFork `{Encode A, Encode B} {ζ}
     P μ (φ : A → iProp Σ) η e1 e2 (φ_arg : B → iProp Σ) :
-    imp^{ι} eval η e1 @ E <|Ψ|> ⟨⟨ ζ ⟩⟩ {{ λ f, iSpec τ[B] f P }} -∗
-    imp^{ι} eval η e2 @ E <|Ψ|> ⟨⟨ ζ ⟩⟩ {{ λ a, φ_arg a }} -∗
+    imp eval η e1 @ E <|Ψ|> ⟨⟨ ζ ⟩⟩ {{ λ f, iSpec τ[B] f P }} -∗
+    imp eval η e2 @ E <|Ψ|> ⟨⟨ ζ ⟩⟩ {{ λ a, φ_arg a }} -∗
     ▷ (∀ ι' a m, isThread ι' μ φ -∗ φ_arg a -∗
-                 P a m -∗ imp^{ι'} m @ E <| ⊥ |> ⟨⟨ λ e, □ μ e ⟩⟩ {{ λ o, □ φ o }}) -∗
-    imp^{ι} eval η (EFork e1 e2) @ E <|Ψ|> ⟨⟨ ζ ⟩⟩ {{ λ ι, isThread ι μ φ }}.
+                 P a m -∗ imp m @ E <| ⊥ |> ⟨⟨ λ e, □ μ e ⟩⟩ {{ λ o, □ φ o }}) -∗
+    imp eval η (EFork e1 e2) @ E <|Ψ|> ⟨⟨ ζ ⟩⟩ {{ λ ι, isThread ι μ φ }}.
   Proof.
     iIntros "H1 H2 Hcall".
     iApply (imp_EFork' with "H1 H2").
@@ -941,11 +951,11 @@ Section imp_rules_expr.
   (* Rule for fork when the postcondition of the spawned thread is persistent *)
   Local Lemma imp_EFork_persistent' `{Encode B} {ζ}
     (Φ1 : val → iProp Σ) (Φ2 : B → iProp Σ) (φ : iProp Σ) η e1 e2 :
-    imp^{ι} eval η e1 @ E <|Ψ|> ⟨⟨ ζ ⟩⟩ {{ Φ1 }} -∗
-    imp^{ι} eval η e2 @ E <|Ψ|> ⟨⟨ ζ ⟩⟩ {{ Φ2 }} -∗
-    ▷ (∀ ι' v1 v2, Φ1 v1 -∗ Φ2 v2 -∗
-                  imp^{ι'} call v1 #v2 @ E <|⊥|> {{ λ (_ : B), □ φ }}) -∗
-    imp^{ι} eval η (EFork e1 e2) @ E <|Ψ|> ⟨⟨ ζ ⟩⟩ {{ λ ι', □ joinable B ι' φ }}.
+    imp eval η e1 @ E <|Ψ|> ⟨⟨ ζ ⟩⟩ {{ Φ1 }} -∗
+    imp eval η e2 @ E <|Ψ|> ⟨⟨ ζ ⟩⟩ {{ Φ2 }} -∗
+    ▷ (∀ v1 v2, Φ1 v1 -∗ Φ2 v2 -∗
+                  imp call v1 #v2 @ E <|⊥|> {{ λ (_ : B), □ φ }}) -∗
+    imp eval η (EFork e1 e2) @ E <|Ψ|> ⟨⟨ ζ ⟩⟩ {{ λ ι', □ joinable B ι' φ }}.
   Proof.
     iIntros "H1 H2 Hcall". simpl_eval.
     iApply (imp_Par _ _ _ _ _ _ (pfbind inject2 (λ '(f, v), fork f v)) with "H1 H2").
@@ -971,15 +981,15 @@ Section imp_rules_expr.
 
   Lemma imp_EFork_persistent `{Encode A} {ζ}
     φ P η e1 e2 (φ_arg : A → iProp Σ) :
-    imp^{ι} eval η e1 @ E <|Ψ|> ⟨⟨ ζ ⟩⟩ {{ λ f, iSpec τ[A] f P }} -∗
-    imp^{ι} eval η e2 @ E <|Ψ|> ⟨⟨ ζ ⟩⟩ {{ φ_arg }} -∗
-    ▷ (∀ ι' a m, φ_arg a -∗
-                 P a m -∗ imp^{ι'} m @ E <|⊥|> {{ λ (_ : A), □ φ }}) -∗
-    imp^{ι} eval η (EFork e1 e2) @ E <|Ψ|> ⟨⟨ ζ ⟩⟩ {{ λ ι', □ joinable A ι' φ }}.
+    imp eval η e1 @ E <|Ψ|> ⟨⟨ ζ ⟩⟩ {{ λ f, iSpec τ[A] f P }} -∗
+    imp eval η e2 @ E <|Ψ|> ⟨⟨ ζ ⟩⟩ {{ φ_arg }} -∗
+    ▷ (∀ a m, φ_arg a -∗
+                 P a m -∗ imp m @ E <|⊥|> {{ λ (_ : A), □ φ }}) -∗
+    imp eval η (EFork e1 e2) @ E <|Ψ|> ⟨⟨ ζ ⟩⟩ {{ λ ι', □ joinable A ι' φ }}.
   Proof.
     iIntros "H1 H2 Hcall".
     iApply (imp_EFork_persistent' with "H1 H2").
-    iIntros "!>" (ι' f v) "HSpec H2"; simpl.
+    iIntros "!>" (f v) "HSpec H2"; simpl.
     iApply ("Hcall" with "H2").
     rewrite iSpec_equation_1.
     iApply "HSpec".
@@ -989,11 +999,11 @@ Section imp_rules_expr.
   resources that other threads can recover when joining. *)
   Local Lemma imp_EFork_resourceful_list' `{Encode B} {ζ}
     (Φ1 : val → iProp Σ) (Φ2 : B → iProp Σ) φs η e1 e2 :
-    imp^{ι} eval η e1 @ E <|Ψ|> ⟨⟨ ζ ⟩⟩ {{ Φ1 }} -∗
-    imp^{ι} eval η e2 @ E <|Ψ|> ⟨⟨ ζ ⟩⟩ {{ Φ2 }} -∗
-    ▷ (∀ ι' v1 v2, Φ1 v1 -∗ Φ2 v2 -∗
-                  imp^{ι'} call v1 #v2 @ E <|⊥|> {{ λ (_ : B), [∗ list] φ ∈ φs, φ }}) -∗
-    imp^{ι} eval η (EFork e1 e2) @ E <|Ψ|> ⟨⟨ ζ ⟩⟩ {{ λ ι', [∗ list] φ ∈ φs, joinable B ι' φ }}.
+    imp eval η e1 @ E <|Ψ|> ⟨⟨ ζ ⟩⟩ {{ Φ1 }} -∗
+    imp eval η e2 @ E <|Ψ|> ⟨⟨ ζ ⟩⟩ {{ Φ2 }} -∗
+    ▷ (∀ v1 v2, Φ1 v1 -∗ Φ2 v2 -∗
+                  imp call v1 #v2 @ E <|⊥|> {{ λ (_ : B), [∗ list] φ ∈ φs, φ }}) -∗
+    imp eval η (EFork e1 e2) @ E <|Ψ|> ⟨⟨ ζ ⟩⟩ {{ λ ι', [∗ list] φ ∈ φs, joinable B ι' φ }}.
   Proof.
     (* TODO reuse the proof from [stop_rules.v] instead of having this one, which is now redundant *)
     iIntros "H1 H2 Hcall". simpl_eval.
@@ -1012,16 +1022,16 @@ Section imp_rules_expr.
 
   Lemma imp_EFork_resourceful_list `{Encode A} {ζ}
     φs P η e1 e2 (φ_arg : A → iProp Σ) :
-    imp^{ι} eval η e1 @ E <|Ψ|> ⟨⟨ ζ ⟩⟩ {{ λ f, iSpec τ[A] f P }} -∗
-    imp^{ι} eval η e2 @ E <|Ψ|> ⟨⟨ ζ ⟩⟩ {{ λ a, φ_arg a }} -∗
-    ▷ (∀ ι' a m, φ_arg a -∗
-                 P a m -∗ imp^{ι'} m @ E <| ⊥ |> {{ λ (_ : A), [∗ list] φ ∈ φs, φ }}) -∗
-    imp^{ι} eval η (EFork e1 e2) @ E <|Ψ|> ⟨⟨ ζ ⟩⟩ {{ λ ι', [∗ list] φ ∈ φs, joinable A ι' φ }}.
+    imp eval η e1 @ E <|Ψ|> ⟨⟨ ζ ⟩⟩ {{ λ f, iSpec τ[A] f P }} -∗
+    imp eval η e2 @ E <|Ψ|> ⟨⟨ ζ ⟩⟩ {{ λ a, φ_arg a }} -∗
+    ▷ (∀ a m, φ_arg a -∗
+                 P a m -∗ imp m @ E <| ⊥ |> {{ λ (_ : A), [∗ list] φ ∈ φs, φ }}) -∗
+    imp eval η (EFork e1 e2) @ E <|Ψ|> ⟨⟨ ζ ⟩⟩ {{ λ ι', [∗ list] φ ∈ φs, joinable A ι' φ }}.
   Proof.
     (* TODO reuse the proof from [stop_rules.v] instead of having this one, which is now redundant *)
     iIntros "H1 H2 Hcall".
     iApply (imp_EFork_resourceful_list' with "H1 H2").
-    iIntros "!>" (ι' f v) "HSpec H2"; simpl.
+    iIntros "!>" (f v) "HSpec H2"; simpl.
     iApply ("Hcall" with "H2").
     rewrite iSpec_equation_1.
     iApply "HSpec".
@@ -1031,15 +1041,15 @@ Section imp_rules_expr.
 
   Local Lemma imp_EFork_one_resource `{Encode A} {ζ}
     φ P η e1 e2 (φ_arg : A → iProp Σ) :
-    imp^{ι} eval η e1 @ E <|Ψ|> ⟨⟨ ζ ⟩⟩ {{ λ f, iSpec τ[A] f P }} -∗
-    imp^{ι} eval η e2 @ E <|Ψ|> ⟨⟨ ζ ⟩⟩ {{ λ a, φ_arg a }} -∗
-    ▷ (∀ ι' a m, φ_arg a -∗ P a m -∗ imp^{ι'} m @ E <| ⊥ |> {{ λ (_ : A), φ }}) -∗
-    imp^{ι} eval η (EFork e1 e2) @ E <|Ψ|> ⟨⟨ ζ ⟩⟩ {{ λ ι', joinable A ι' φ }}.
+    imp eval η e1 @ E <|Ψ|> ⟨⟨ ζ ⟩⟩ {{ λ f, iSpec τ[A] f P }} -∗
+    imp eval η e2 @ E <|Ψ|> ⟨⟨ ζ ⟩⟩ {{ λ a, φ_arg a }} -∗
+    ▷ (∀ a m, φ_arg a -∗ P a m -∗ imp m @ E <| ⊥ |> {{ λ (_ : A), φ }}) -∗
+    imp eval η (EFork e1 e2) @ E <|Ψ|> ⟨⟨ ζ ⟩⟩ {{ λ ι', joinable A ι' φ }}.
   Proof.
     iIntros "H1 H2 H".
     iApply (imp_mono_ret _ (eval η (EFork e1 e2)) with "[-]").
     iApply (imp_EFork_resourceful_list [φ] with "H1 H2 [H]").
-    - iIntros "!> % % % H1 H2".
+    - iIntros "!> % % H1 H2".
       iSpecialize ("H" with "H1 H2").
       iApply (imp_mono_ret with "H").
       iIntros (_) "/= $".
@@ -1048,15 +1058,15 @@ Section imp_rules_expr.
 
   Local Lemma imp_EFork_two_resources `{Encode A} {ζ}
     φ1 φ2 P η e1 e2 (φ_arg : A → iProp Σ) :
-    imp^{ι} eval η e1 @ E <|Ψ|> ⟨⟨ ζ ⟩⟩ {{ λ f, iSpec τ[A] f P }} -∗
-    imp^{ι} eval η e2 @ E <|Ψ|> ⟨⟨ ζ ⟩⟩ {{ λ a, φ_arg a }} -∗
-    ▷ (∀ ι' a m, φ_arg a -∗ P a m -∗ imp^{ι'} m @ E <|⊥|> {{ λ (_ : A), φ1 ∗ φ2 }}) -∗
-    imp^{ι} eval η (EFork e1 e2) @ E <|Ψ|> ⟨⟨ ζ ⟩⟩ {{ λ ι', joinable A ι' φ1 ∗ joinable A ι' φ2 }}.
+    imp eval η e1 @ E <|Ψ|> ⟨⟨ ζ ⟩⟩ {{ λ f, iSpec τ[A] f P }} -∗
+    imp eval η e2 @ E <|Ψ|> ⟨⟨ ζ ⟩⟩ {{ λ a, φ_arg a }} -∗
+    ▷ (∀ a m, φ_arg a -∗ P a m -∗ imp m @ E <|⊥|> {{ λ (_ : A), φ1 ∗ φ2 }}) -∗
+    imp eval η (EFork e1 e2) @ E <|Ψ|> ⟨⟨ ζ ⟩⟩ {{ λ ι', joinable A ι' φ1 ∗ joinable A ι' φ2 }}.
   Proof.
     iIntros "H1 H2 H".
     iApply (imp_mono_ret _ (eval η (EFork e1 e2)) with "[-]").
     iApply (imp_EFork_resourceful_list [φ1; φ2] with "H1 H2 [H]").
-    - iIntros "!> % % % H1 H2".
+    - iIntros "!> % % H1 H2".
       iSpecialize ("H" with "H1 H2").
       iApply (imp_mono_ret with "H").
       iIntros (_) "/= ($ & $)".
@@ -1064,9 +1074,9 @@ Section imp_rules_expr.
   Qed.
 
   Lemma imp_EJoin2 `{Encode A} {ζ} e η μ (φ : A → iProp Σ) Φ :
-    imp^{ι} eval η e @ E <|Ψ|> ⟨⟨ ζ ⟩⟩ {{ λ ι, isThread ι μ φ }} -∗
+    imp eval η e @ E <|Ψ|> ⟨⟨ ζ ⟩⟩ {{ λ ι, isThread ι μ φ }} -∗
     ▷ (∀ x, □ φ x -∗ Φ x) ∧ ▷ (∀ e : exn, □ μ e -∗ ζ e) -∗
-    imp^{ι} eval η (EJoin e) @ E <|Ψ|> ⟨⟨ ζ ⟩⟩ {{ Φ }}.
+    imp eval η (EJoin e) @ E <|Ψ|> ⟨⟨ ζ ⟩⟩ {{ Φ }}.
   Proof.
     iIntros "Hid Hjoined". simpl_eval.
     iApply (imp_bind _ _ (λ t, join t) with "[Hid]").
@@ -1080,9 +1090,9 @@ Section imp_rules_expr.
   Qed.
 
   Lemma imp_EJoin `{Encode A} {ζ} e η (φ : A → iProp Σ) Φ :
-    imp^{ι} eval η e @ E <|Ψ|> ⟨⟨ ζ ⟩⟩ {{ λ ι, isThread ι ⊥ φ }} -∗
+    imp eval η e @ E <|Ψ|> ⟨⟨ ζ ⟩⟩ {{ λ ι, isThread ι ⊥ φ }} -∗
     ▷ (∀ x, □ φ x -∗ Φ x) -∗
-    imp^{ι} eval η (EJoin e) @ E <|Ψ|> ⟨⟨ ζ ⟩⟩ {{ Φ }}.
+    imp eval η (EJoin e) @ E <|Ψ|> ⟨⟨ ζ ⟩⟩ {{ Φ }}.
   Proof.
     iIntros "Hid Hjoined".
     iApply (imp_EJoin2 with "Hid").
@@ -1094,9 +1104,9 @@ Section imp_rules_expr.
   (* The joinable rule for join is the same for persistent and resourceful posts *)
   Lemma imp_EJoin_joinable `{Encode A} {ζ} e η φ (Φ : A → iProp Σ) :
     ↑joinN ⊆ E →
-    imp^{ι} eval η e @ E <|Ψ|> ⟨⟨ ζ ⟩⟩ {{ λ ι', joinable A ι' φ }} -∗
+    imp eval η e @ E <|Ψ|> ⟨⟨ ζ ⟩⟩ {{ λ ι', joinable A ι' φ }} -∗
     ▷ (∀ x, ▷ φ -∗ Φ x) ∧ ▷ (∀ e, ▷ φ -∗ ζ e) -∗
-    imp^{ι} eval η (EJoin e) @ E <|Ψ|> ⟨⟨ ζ ⟩⟩ {{ Φ }}.
+    imp eval η (EJoin e) @ E <|Ψ|> ⟨⟨ ζ ⟩⟩ {{ Φ }}.
   Proof.
     iIntros "%Hmask Hid Hjoined". simpl_eval.
     iApply (imp_bind _ _ (λ t, join t) with "[Hid]").
