rocq-osiris/theories/program_logic/reasoning_rules/impure_rules.v
@@ -13,12 +13,12 @@ Section micro_combinators.
   Context `{!osirisGS Σ}.
 
   Context {A V X : Type} `{Observe A V}.
-  Context {ι : thread} {E : coPset} {Ψ : iEff Σ} {ζ : X → iProp Σ} {Φ : A → iProp Σ}.
+  Context {E : coPset} {Ψ : iEff Σ} {ζ : X → iProp Σ} {Φ : A → iProp Σ}.
 
   Lemma imp_ret (v : V) a :
     v = ♯ a →
     Φ a -∗
-    imp^{ι} (ret v) @ E <|Ψ|> ⟨⟨ ζ ⟩⟩ {{ Φ }}.
+    imp (ret v) @ E <|Ψ|> ⟨⟨ ζ ⟩⟩ {{ Φ }}.
   Proof.
     iIntros (Hobserve) "HΦ".
     iApply ewp_ret.
@@ -26,7 +26,7 @@ Section micro_combinators.
   Qed.
 
   Lemma invert_imp_ret (v : V) :
-    imp^{ι} (ret v) @ E <|Ψ|> ⟨⟨ ζ ⟩⟩ {{ Φ }} -∗
+    imp (ret v) @ E <|Ψ|> ⟨⟨ ζ ⟩⟩ {{ Φ }} -∗
     |={E}=> ∃ a, ⌜v = ♯a⌝ ∗ Φ a.
   Proof.
     iIntros "Himp".
@@ -36,7 +36,7 @@ Section micro_combinators.
 
   Lemma imp_throw e :
     ζ e -∗
-    imp^{ι} (throw e) @ E <|Ψ|> ⟨⟨ ζ ⟩⟩ {{ Φ }}.
+    imp (throw e) @ E <|Ψ|> ⟨⟨ ζ ⟩⟩ {{ Φ }}.
   Proof.
     iIntros "Hζ".
     iApply ewp_throw.
@@ -44,7 +44,7 @@ Section micro_combinators.
   Qed.
 
   Lemma invert_imp_throw e :
-    imp^{ι} (throw e) @ E <|Ψ|> ⟨⟨ ζ ⟩⟩ {{ Φ }} -∗
+    imp (throw e) @ E <|Ψ|> ⟨⟨ ζ ⟩⟩ {{ Φ }} -∗
     |={E}=> ζ e.
   Proof.
     iIntros "Himp".
@@ -53,7 +53,7 @@ Section micro_combinators.
   Qed.
 
   Lemma invert_imp_Crash :
-    imp^{ι} Crash @ E <|Ψ|> ⟨⟨ ζ ⟩⟩ {{ Φ }} -∗
+    imp Crash @ E <|Ψ|> ⟨⟨ ζ ⟩⟩ {{ Φ }} -∗
     |={E}=> False.
   Proof.
     iIntros "Himp".
@@ -64,10 +64,10 @@ Section micro_combinators.
   Lemma imp_try2 `{Observe A1 V1} {X1}
     (Φ' : A1 → iProp Σ) (ζ' : X1 → iProp Σ) (m : micro V1 X1)
     (h : outcome2 V1 X1 -> micro V X) :
-    imp^{ι} m @ E <|Ψ|> ⟨⟨ ζ' ⟩⟩ {{ Φ' }} -∗
-    (∀ a, Φ' a -∗ imp^{ι} (continue h ♯a) @ E <|Ψ|> ⟨⟨ ζ ⟩⟩ {{ Φ }}) ∧
-    (∀ e, ζ' e -∗ imp^{ι} (discontinue h e) @ E <|Ψ|> ⟨⟨ ζ ⟩⟩ {{ Φ }}) -∗
-    imp^{ι} (try2 m h) @ E <|Ψ|> ⟨⟨ ζ ⟩⟩ {{ Φ }}.
+    imp m @ E <|Ψ|> ⟨⟨ ζ' ⟩⟩ {{ Φ' }} -∗
+    (∀ a, Φ' a -∗ imp (continue h ♯a) @ E <|Ψ|> ⟨⟨ ζ ⟩⟩ {{ Φ }}) ∧
+    (∀ e, ζ' e -∗ imp (discontinue h e) @ E <|Ψ|> ⟨⟨ ζ ⟩⟩ {{ Φ }}) -∗
+    imp (try2 m h) @ E <|Ψ|> ⟨⟨ ζ ⟩⟩ {{ Φ }}.
   Proof.
     iIntros "Himp Hresume".
     iApply ewp_try2.
@@ -80,10 +80,10 @@ Section micro_combinators.
   Lemma imp_try `{Observe A1 V1} {X1}
     (Φ' : A1 → iProp Σ) (ζ' : X1 → iProp Σ) (m : micro V1 X1)
     (k : V1 → micro V X) (z : X1 → micro V X) :
-    imp^{ι} m @ E <|Ψ|> ⟨⟨ ζ' ⟩⟩ {{ Φ' }} -∗
-    (∀ a, Φ' a -∗ imp^{ι} (k ♯a) @ E <|Ψ|> ⟨⟨ ζ ⟩⟩ {{ Φ }}) ∧
-    (∀ e, ζ' e -∗ imp^{ι} (z e) @ E <|Ψ|> ⟨⟨ ζ ⟩⟩ {{ Φ }}) -∗
-    imp^{ι} (try m k z) @ E <|Ψ|> ⟨⟨ ζ ⟩⟩ {{ Φ }}.
+    imp m @ E <|Ψ|> ⟨⟨ ζ' ⟩⟩ {{ Φ' }} -∗
+    (∀ a, Φ' a -∗ imp (k ♯a) @ E <|Ψ|> ⟨⟨ ζ ⟩⟩ {{ Φ }}) ∧
+    (∀ e, ζ' e -∗ imp (z e) @ E <|Ψ|> ⟨⟨ ζ ⟩⟩ {{ Φ }}) -∗
+    imp (try m k z) @ E <|Ψ|> ⟨⟨ ζ ⟩⟩ {{ Φ }}.
   Proof.
     iIntros "Himp Hresume".
     iApply (imp_try2 with "Himp [Hresume]").
@@ -94,9 +94,9 @@ Section micro_combinators.
   Lemma imp_bind `{Observe A1 V1}
     (Φ' : A1 → iProp Σ) (m : micro V1 X)
     (f : V1 → micro V X) :
-    imp^{ι} m @ E <|Ψ|> ⟨⟨ ζ ⟩⟩ {{ Φ' }} -∗
-    (∀ (x : A1), Φ' x -∗ imp^{ι} (f ♯x) @ E <|Ψ|> ⟨⟨ ζ ⟩⟩ {{ Φ }}) -∗
-    imp^{ι} (bind m f) @ E <|Ψ|> ⟨⟨ ζ ⟩⟩ {{ Φ }}.
+    imp m @ E <|Ψ|> ⟨⟨ ζ ⟩⟩ {{ Φ' }} -∗
+    (∀ (x : A1), Φ' x -∗ imp (f ♯x) @ E <|Ψ|> ⟨⟨ ζ ⟩⟩ {{ Φ }}) -∗
+    imp (bind m f) @ E <|Ψ|> ⟨⟨ ζ ⟩⟩ {{ Φ }}.
   Proof.
     iIntros "Himp Hconseq".
     rewrite bind_as_try.
@@ -108,10 +108,10 @@ Section micro_combinators.
   Lemma imp_bind2 `{Observe A1 V1}
     (Φ' : A1 → iProp Σ) (ζ' : X → iProp Σ) (m : micro V1 X)
     (f : V1 → micro V X) :
-    imp^{ι} m @ E <|Ψ|> ⟨⟨ ζ' ⟩⟩ {{ Φ' }} -∗
-    (∀ (x : A1), Φ' x -∗ imp^{ι} (f ♯x) @ E <|Ψ|> ⟨⟨ ζ ⟩⟩ {{ Φ }}) ∧
+    imp m @ E <|Ψ|> ⟨⟨ ζ' ⟩⟩ {{ Φ' }} -∗
+    (∀ (x : A1), Φ' x -∗ imp (f ♯x) @ E <|Ψ|> ⟨⟨ ζ ⟩⟩ {{ Φ }}) ∧
     (∀ (e : X), ζ' e -∗ ζ e) -∗
-    imp^{ι} (bind m f) @ E <|Ψ|> ⟨⟨ ζ ⟩⟩ {{ Φ }}.
+    imp (bind m f) @ E <|Ψ|> ⟨⟨ ζ ⟩⟩ {{ Φ }}.
   Proof.
     iIntros "Himp Hconseq".
     rewrite bind_as_try.
@@ -124,8 +124,8 @@ Section micro_combinators.
   Qed.
 
   Lemma imp_widen (m : micro V void) :
-    imp^{ι} m @ E <|Ψ|> {{ Φ }} -∗
-    imp^{ι} (widen m) @ E <|Ψ|> ⟨⟨ ζ ⟩⟩ {{ Φ }}.
+    imp m @ E <|Ψ|> {{ Φ }} -∗
+    imp (widen m) @ E <|Ψ|> ⟨⟨ ζ ⟩⟩ {{ Φ }}.
   Proof.
     iIntros "Himp".
     unfold widen.
@@ -138,12 +138,12 @@ Section micro_combinators.
 
   Lemma imp_Par `{Observe A1 V1} `{Observe A2 V2} {X'}
     Φ1 ζ1 Φ2 ζ2 m1 m2 (k : outcome2 (V1 * V2) X' → micro V X) :
-    imp^{ι} m1 @ E <|Ψ|> ⟨⟨ ζ1 ⟩⟩ {{ Φ1 }} -∗
-    imp^{ι} m2 @ E <|Ψ|> ⟨⟨ ζ2 ⟩⟩ {{ Φ2 }} -∗
-    (∀ e, ζ1 e -∗ ▷ imp^{ι} discontinue k e @ E <|Ψ|> ⟨⟨ ζ ⟩⟩ {{ Φ }}) ∧
-    (∀ e, ζ2 e -∗ ▷ imp^{ι} discontinue k e @ E <|Ψ|> ⟨⟨ ζ ⟩⟩ {{ Φ }}) ∧
-    (∀ x y, Φ1 x -∗ Φ2 y -∗ ▷ imp^{ι} continue k (♯x, ♯y) @ E <|Ψ|> ⟨⟨ ζ ⟩⟩ {{ Φ }}) -∗
-    imp^{ι} (Par m1 m2 k) @ E <|Ψ|> ⟨⟨ ζ ⟩⟩ {{ Φ }}.
+    imp m1 @ E <|Ψ|> ⟨⟨ ζ1 ⟩⟩ {{ Φ1 }} -∗
+    imp m2 @ E <|Ψ|> ⟨⟨ ζ2 ⟩⟩ {{ Φ2 }} -∗
+    (∀ e, ζ1 e -∗ ▷ imp discontinue k e @ E <|Ψ|> ⟨⟨ ζ ⟩⟩ {{ Φ }}) ∧
+    (∀ e, ζ2 e -∗ ▷ imp discontinue k e @ E <|Ψ|> ⟨⟨ ζ ⟩⟩ {{ Φ }}) ∧
+    (∀ x y, Φ1 x -∗ Φ2 y -∗ ▷ imp continue k (♯x, ♯y) @ E <|Ψ|> ⟨⟨ ζ ⟩⟩ {{ Φ }}) -∗
+    imp (Par m1 m2 k) @ E <|Ψ|> ⟨⟨ ζ ⟩⟩ {{ Φ }}.
   Proof.
     iIntros "H1 H2 Hjoin".
     iApply (ewp_Par with "H1 H2").
@@ -156,10 +156,10 @@ Section micro_combinators.
 
   Lemma imp_Par2 `{Observe A1 V1} `{Observe A2 V2} {X'}
     Φ1 Φ2 m1 m2 (k : outcome2 (V1 * V2) X' → micro V X) :
-    imp^{ι} m1 @ E <|Ψ|> {{ Φ1 }} -∗
-    imp^{ι} m2 @ E <|Ψ|> {{ Φ2 }} -∗
-    (∀ x y, Φ1 x -∗ Φ2 y -∗ ▷ imp^{ι} continue k (♯x, ♯y) @ E <|Ψ|> ⟨⟨ ζ ⟩⟩ {{ Φ }}) -∗
-    imp^{ι} (Par m1 m2 k) @ E <|Ψ|> ⟨⟨ ζ ⟩⟩ {{ Φ }}.
+    imp m1 @ E <|Ψ|> {{ Φ1 }} -∗
+    imp m2 @ E <|Ψ|> {{ Φ2 }} -∗
+    (∀ x y, Φ1 x -∗ Φ2 y -∗ ▷ imp continue k (♯x, ♯y) @ E <|Ψ|> ⟨⟨ ζ ⟩⟩ {{ Φ }}) -∗
+    imp (Par m1 m2 k) @ E <|Ψ|> ⟨⟨ ζ ⟩⟩ {{ Φ }}.
   Proof.
     iIntros "H1 H2 Hjoin".
     iApply (imp_Par with "H1 H2 [Hjoin]").
@@ -177,11 +177,11 @@ Section micro_codes.
 
   Context `{!osirisGS Σ}.
   Context {V : Type} `{Observe A V}.
-  Context {ι : thread} {E : coPset} {Ψ : iEff Σ} {Φ : A → iProp Σ}.
+  Context {E : coPset} {Ψ : iEff Σ} {Φ : A → iProp Σ}.
 
   Lemma imp_please {ζ} η e :
-    ▷ imp^{ι} eval η e @ E <|Ψ|> ⟨⟨ ζ ⟩⟩ {{ Φ }} -∗
-    imp^{ι} please_eval η e @ E <|Ψ|> ⟨⟨ ζ ⟩⟩ {{ Φ }}.
+    ▷ imp eval η e @ E <|Ψ|> ⟨⟨ ζ ⟩⟩ {{ Φ }} -∗
+    imp please_eval η e @ E <|Ψ|> ⟨⟨ ζ ⟩⟩ {{ Φ }}.
   Proof.
     iIntros "Himp".
     rewrite /please_eval.
@@ -193,8 +193,8 @@ Section micro_codes.
   Qed.
 
   Lemma imp_choose {ζ} (m1 m2 : micro V exn) :
-    imp^{ι} m1 @ E <|Ψ|> ⟨⟨ ζ ⟩⟩ {{ Φ }} ∧ imp^{ι} m2 @ E <|Ψ|> ⟨⟨ ζ ⟩⟩ {{ Φ }} -∗
-    imp^{ι} (code.choose m1 m2) @ E <|Ψ|> ⟨⟨ ζ ⟩⟩ {{ Φ }}.
+    imp m1 @ E <|Ψ|> ⟨⟨ ζ ⟩⟩ {{ Φ }} ∧ imp m2 @ E <|Ψ|> ⟨⟨ ζ ⟩⟩ {{ Φ }} -∗
+    imp (code.choose m1 m2) @ E <|Ψ|> ⟨⟨ ζ ⟩⟩ {{ Φ }}.
   Proof.
     iIntros "Hm". rewrite /code.choose /code.flip.
     iApply (imp_bind (λ (b : bool), True)%I (stop CFlip ())).
@@ -218,13 +218,13 @@ Section monotonicity.
   Context `{!osirisGS Σ}.
 
   Context {A V X : Type} `{Observe A V}.
-  Context {ι : thread} {E : coPset} {Ψ : iEff Σ} {ζ : X → iProp Σ} {Φ : A → iProp Σ}.
+  Context {E : coPset} {Ψ : iEff Σ} {ζ : X → iProp Σ} {Φ : A → iProp Σ}.
 
   Lemma imp_mono (Φ' : A → iProp Σ) (ζ' : X → iProp Σ) m :
-    imp^{ι} m @ E <|Ψ|> ⟨⟨ ζ' ⟩⟩ {{ Φ' }} -∗
+    imp m @ E <|Ψ|> ⟨⟨ ζ' ⟩⟩ {{ Φ' }} -∗
     (∀ (x : A), Φ' x -∗ Φ x) -∗
     (∀ (e : X), ζ' e -∗ ζ e) -∗
-    imp^{ι} m @ E <|Ψ|> ⟨⟨ ζ ⟩⟩ {{ Φ }}.
+    imp m @ E <|Ψ|> ⟨⟨ ζ ⟩⟩ {{ Φ }}.
   Proof.
     iIntros "Himp Hmonor Hmonot".
     iApply (ewp_mono with "Himp").
@@ -237,9 +237,9 @@ Section monotonicity.
   Qed.
 
   Lemma imp_mono_ret (Φ' : A → iProp Σ) m :
-    imp^{ι} m @ E <|Ψ|> ⟨⟨ ζ ⟩⟩ {{ Φ' }} -∗
+    imp m @ E <|Ψ|> ⟨⟨ ζ ⟩⟩ {{ Φ' }} -∗
     (∀ (x : A), Φ' x -∗ Φ x) -∗
-    imp^{ι} m @ E <|Ψ|> ⟨⟨ ζ ⟩⟩ {{ Φ }}.
+    imp m @ E <|Ψ|> ⟨⟨ ζ ⟩⟩ {{ Φ }}.
   Proof.
     iIntros "Himp Hmono".
     iApply (ewp_mono with "Himp").
@@ -250,9 +250,9 @@ Section monotonicity.
   Qed.
 
   Lemma imp_mono_throw (ζ' : X → iProp Σ) m :
-    imp^{ι} m @ E <|Ψ|> ⟨⟨ ζ' ⟩⟩ {{ Φ }} -∗
+    imp m @ E <|Ψ|> ⟨⟨ ζ' ⟩⟩ {{ Φ }} -∗
     (∀ (e : X), ζ' e -∗ ζ e) -∗
-    imp^{ι} m @ E <|Ψ|> ⟨⟨ ζ ⟩⟩ {{ Φ }}.
+    imp m @ E <|Ψ|> ⟨⟨ ζ ⟩⟩ {{ Φ }}.
   Proof.
     iIntros "Himp Hmono".
     iApply (ewp_mono with "Himp").
@@ -262,18 +262,18 @@ Section monotonicity.
   Qed.
 
   Lemma imp_mono_prot Ψ' m :
-    imp^{ι} m @ E <|Ψ'|> ⟨⟨ ζ ⟩⟩ {{ Φ }} -∗
+    imp m @ E <|Ψ'|> ⟨⟨ ζ ⟩⟩ {{ Φ }} -∗
     (Ψ' ⊑ Ψ)%ieff -∗
-    imp^{ι} m @ E <|Ψ|> ⟨⟨ ζ ⟩⟩ {{ Φ }}.
+    imp m @ E <|Ψ|> ⟨⟨ ζ ⟩⟩ {{ Φ }}.
   Proof.
     iIntros "Himp Hmono".
     iApply (ewp_prot_mono with "Hmono Himp").
   Qed.
 
   Lemma imp_mono_pers Φ' m :
-    imp^{ι} m @ E <|Ψ|> ⟨⟨ ζ ⟩⟩ {{ Φ' }} -∗
+    imp m @ E <|Ψ|> ⟨⟨ ζ ⟩⟩ {{ Φ' }} -∗
     □ (∀ x, Φ' x ={E}=∗ Φ x) -∗
-    imp^{ι} m @ E <|Ψ|> ⟨⟨ ζ ⟩⟩ {{ Φ }}.
+    imp m @ E <|Ψ|> ⟨⟨ ζ ⟩⟩ {{ Φ }}.
   Proof.
     iIntros "Himp #Hmono".
     iApply (ewp_pers_mono with "Himp").
@@ -291,18 +291,18 @@ Section updates.
   Context `{!osirisGS Σ}.
 
   Context {A V X : Type} `{Observe A V}.
-  Context {ι : thread} {E : coPset} {Ψ : iEff Σ} {ζ : X → iProp Σ} {Φ : A → iProp Σ}.
+  Context {E : coPset} {Ψ : iEff Σ} {ζ : X → iProp Σ} {Φ : A → iProp Σ}.
 
   Lemma imp_fupd m :
-    (|={E}=> imp^{ι} m @ E <|Ψ|> ⟨⟨ ζ ⟩⟩ {{ Φ }}) -∗
-    imp^{ι} m @ E <|Ψ|> ⟨⟨ ζ ⟩⟩ {{ Φ }}.
+    (|={E}=> imp m @ E <|Ψ|> ⟨⟨ ζ ⟩⟩ {{ Φ }}) -∗
+    imp m @ E <|Ψ|> ⟨⟨ ζ ⟩⟩ {{ Φ }}.
   Proof.
     iApply ewp_fupd.
   Qed.
 
   Lemma imp_fupd_post m :
-    imp^{ι} m @ E <|Ψ|> ⟨⟨ ζ ⟩⟩ {{ λ x, |={E}=> Φ x }} -∗
-    imp^{ι} m @ E <|Ψ|> ⟨⟨ ζ ⟩⟩ {{ Φ }}.
+    imp m @ E <|Ψ|> ⟨⟨ ζ ⟩⟩ {{ λ x, |={E}=> Φ x }} -∗
+    imp m @ E <|Ψ|> ⟨⟨ ζ ⟩⟩ {{ Φ }}.
   Proof.
     iIntros "Himp".
     iApply ewp_fupd_post.
@@ -312,8 +312,8 @@ Section updates.
   Qed.
 
   Lemma imp_fupd_post2 m :
-    imp^{ι} m @ E <|Ψ|> ⟨⟨ λ e, |={E}=> ζ e ⟩⟩ {{ Φ }} -∗
-    imp^{ι} m @ E <|Ψ|> ⟨⟨ ζ ⟩⟩ {{ Φ }}.
+    imp m @ E <|Ψ|> ⟨⟨ λ e, |={E}=> ζ e ⟩⟩ {{ Φ }} -∗
+    imp m @ E <|Ψ|> ⟨⟨ ζ ⟩⟩ {{ Φ }}.
   Proof.
     iIntros "Himp".
     iApply ewp_fupd_post.
@@ -324,13 +324,24 @@ Section updates.
 
 End updates.
 
-Lemma impure_pure `{osirisGS Σ} {V} `{Observe A V} {X} (m : micro V X) ζ Φ :
+Lemma impure_pure2 `{osirisGS Σ} {V} `{Observe A V} {X} (m : micro V X) ζ Φ :
   pure m Φ ζ →
   ⊢ imp m ⟨⟨ λ e, ⌜ζ e⌝ ⟩⟩ {{ λ x, ⌜Φ x⌝ }}.
 Proof.
   iIntros (Hpure).
-  iIntros (ι).
-  iPoseProof (pure_ewp _ _ _ _ _ _ Hpure) as "Hewp".
+  iPoseProof (pure_ewp _ _ _ _ _ Hpure) as "Hewp".
+  iApply (ewp_mono with "Hewp").
+  iIntros ([|]); last auto.
+  iIntros "(%v & %Henc & %HΦ)".
+  iExists v; iFrame "%".
+Qed.
+
+Lemma impure_pure `{osirisGS Σ} {V} `{Observe A V} {X} (m : micro V X) Φ :
+  pure m Φ ⊥ →
+  ⊢ imp m {{ λ x, ⌜Φ x⌝ }}.
+Proof.
+  iIntros (Hpure).
+  iPoseProof (pure_ewp _ _ _ _ _ Hpure) as "Hewp".
   iApply (ewp_mono with "Hewp").
   iIntros ([|]); last auto.
   iIntros "(%v & %Henc & %HΦ)".
